\documentclass{article}
\usepackage[english]{babel} % To obtain English text with the blindtext package
\usepackage{blindtext}
\begin{document}
$$
D: x \geq 0 \newline
$$

$$
\sum_{n=1}^{\infty} \left(\sqrt[2n+1]{x}-\sqrt[2n-1]{x}\right) = \left(\sqrt[3]{x} - \sqrt[1]{x} \right) + \left( \sqrt[5]{x} - \sqrt[3]{x} \right) + \dots
$$

$$
\sum_{k=1}^{n} \sqrt[2k+1]{x} - \sum_{k=1}^{n} \sqrt[2k-1]{x} = \sqrt[2n+1]{x} - \sqrt[1]{x} + \sum_{k=1}^{n-1}\sqrt[2k+1]{x} - \sum_{k=2}^{n} \sqrt[2k-1]{x} = \sqrt[2n+1]{x} - \sqrt[1]{x}
$$

$$
\lim_{n \to \infty} \sum_{k=1}^{n} \left( \sqrt[2k+1]{x} - \sqrt[2k-1]{x} \right) = \lim_{n \to \infty}  \sqrt[2n+1]{x} - \sqrt[1]{x} = 
\begin{enumerate}
   \item 
\end{enumerate}
$$

\end{document}