## Pochodne
$$
\begin{array}{l}
(1)& \frac{d}{dx} (uv) &=& \frac{du}{dx} v + u \frac{dv}{dx} \\
(2)& \frac{d}{dx} \left( \frac{u}{v} \right) &=& \frac{\frac{du}{dx} v - u \frac{dv}{dx}}{v^2} \\
(3)& \frac{dy}{dx} &=& \frac{dy}{du} \frac{du}{dx} \\
(4)& \frac{d}{dx} x^n &=& n x^{n-1} \\
(5)& \frac{d}{dx} a^x &=& a^x \ln a \\
(6)& \frac{d}{dx} e^x &=& e^x \\
(7)& \frac{d}{dx} \log_{a}{x} &=& \frac{1}{x \ln a} \\
(8)& \frac{d}{dx} \ln x &=& \frac{1}{x} \\
(9)& \frac{d}{dx} \sin x &=& \cos x \\
(10)& \frac{d}{dx} \cos x &=& - \sin x \\
(11)& \frac{d}{dx} \tan x &=& \sec^2 x \\
(12)& \frac{d}{dx} \cot x &=& - \csc^2 x  \\
(13)& \frac{d}{dx} \sec x &=& \sec x \tan x \\
(14)& \frac{d}{dx} \csc x &=& - \csc x \cot x \\
(15)& \frac{d}{dx} \sin^{-1} x &=& \frac{1}{\sqrt{1 - x^2}} \\
(16)& \frac{d}{dx} \tan^{-1} x &=& \frac{1}{1 + x^2} \\
\end{array}
$$

## Asymptoty

1. Prosta $x = c$ jest asymptota pionowa krzywej gdy, jest jej asymptota lewostronna i prawostronna.
2. 