
| $p$ | $q$ |     |     |     |     |     |
| --- | --- | --- | --- | --- | --- | --- |
| 1   | 1   |     |     |     |     |     |
| 1   | 0   |     |     |     |     |     |
| 0   | 1   |     |     |     |     |     |
| 0   | 0   |     |     |     |     |     |
$p\wedge(q\vee r) \Leftrightarrow (p\wedge q)\vee(p\wedge r)$
$p \vee(q \wedge r) \Leftrightarrow (p \vee q) \wedge (p\vee r)$
~$p \Rightarrow q \Leftrightarrow (p\wedge$~$q)$


| $p$ | $q$ | r   | $q\vee r$ | $p\wedge(q\vee r)$ | $p\wedge q$ | $p\wedge r$ | $(p\wedge q)\vee(p\wedge r)$ | F   |
| --- | --- | --- | --------- | ------------------ | ----------- | ----------- | ---------------------------- | --- |
| 1   | 1   | 1   | 1         | 1                  | 1           | 1           | 1                            | 1   |
| 1   | 1   | 0   | 1         | 1                  | 1           | 0           | 1                            | 1   |
| 1   | 0   | 1   | 1         | 1                  | 0           | 1           | 1                            | 1   |
| 1   | 0   | 0   | 0         | 0                  | 0           | 0           | 0                            | 1   |
| 0   | 1   | 1   | 1         | 0                  | 0           | 0           | 0                            | 1   |
| 0   | 1   | 0   | 0         | 0                  | 0           | 0           | 0                            | 1   |
| 0   | 0   | 1   | 1         | 0                  | 0           | 0           | 0                            | 1   |
| 0   | 0   | 0   | 0         | 0                  | 0           | 0           | 0                            | 1   |
